weiterer Fortschritt

Projects/Lindmar_Joost/BinaryHeapTree.lean
@@ -1,14 +1,13 @@
 import Mathlib.Tactic
-
-
-
+#check Nat.div2Induction
+#check ENat
 inductive BinaryTree (α : Type)
   | leaf : BinaryTree α
   | node : BinaryTree α → α → BinaryTree α → BinaryTree α
 
 namespace BinaryTree
 
-def isMinHeap : BinaryTree ℕ → Prop
+def isMinHeap : BinaryTree ENat → Prop
 | leaf => true
 | node l v r => match l, r with
       | leaf, leaf => true
@@ -16,7 +15,7 @@ def isMinHeap : BinaryTree ℕ → Prop
       | leaf, node _ rv _ => v <= rv ∧ isMinHeap r
       | node _ lv _, node _ rv _ => v <= lv ∧ isMinHeap l ∧ v <= rv ∧ isMinHeap r
 
-def heapify (bt: BinaryTree ℕ): BinaryTree ℕ := match bt with
+def heapify (bt: BinaryTree ENat): BinaryTree ENat := match bt with
 | leaf => bt
 | node l v r => match l, r with
     | leaf, leaf => bt
@@ -29,11 +28,11 @@ def heapify (bt: BinaryTree ℕ): BinaryTree ℕ := match bt with
                                           if v <= rv then bt
                                           else node l rv (heapify (node rl v rr))
 
-def leftAndRightAreMinHeap: (BinaryTree ℕ) →  Prop
+def leftAndRightAreMinHeap: (BinaryTree ENat) →  Prop
 | leaf => true
 | node l _ r => isMinHeap l ∧ isMinHeap r
 
-def rootIsMinOfChildren: (BinaryTree ℕ) →  Prop
+def rootIsMinOfChildren: (BinaryTree ENat) →  Prop
 | leaf => true
 | node l v r => match l, r with
     | leaf, leaf => true
@@ -42,53 +41,59 @@ def rootIsMinOfChildren: (BinaryTree ℕ) →  Prop
     | node _ lv _, node _ rv _ =>  v <= lv ∧ v <= rv
 
 
-lemma minHeapThenLeftAndRightAreMinHeap (bt: BinaryTree ℕ): isMinHeap bt → leftAndRightAreMinHeap bt := by
+lemma minHeapThenLeftAndRightAreMinHeap (bt: BinaryTree ENat): isMinHeap bt → leftAndRightAreMinHeap bt := by
 intro hbt
-fun_induction isMinHeap
-. simp [leftAndRightAreMinHeap]
-. simp [leftAndRightAreMinHeap, isMinHeap]
-. expose_names
-  simp [leftAndRightAreMinHeap, hbt]
-  simp [isMinHeap]
-. expose_names
-  simp [leftAndRightAreMinHeap, hbt]
-  simp [isMinHeap]
-. expose_names
-  simp [leftAndRightAreMinHeap, hbt]
+fun_induction isMinHeap; all_goals (grind [leftAndRightAreMinHeap, isMinHeap])
 
-lemma leftAndRightAreMinHeapAndRootIsMinOfChildrenToMinHeap (bt: BinaryTree ℕ): leftAndRightAreMinHeap bt ∧ rootIsMinOfChildren bt → isMinHeap bt := by
+lemma minHeapThenRootIsMinOfChildren (bt: BinaryTree ENat): isMinHeap bt → rootIsMinOfChildren bt := by
 intro hbt
-fun_induction isMinHeap
-. simp
-. simp
-. simp [rootIsMinOfChildren, leftAndRightAreMinHeap] at hbt
-  simp [hbt]
-. simp [rootIsMinOfChildren, leftAndRightAreMinHeap] at hbt
-  simp [hbt]
-. simp [rootIsMinOfChildren, leftAndRightAreMinHeap] at hbt
-  simp [hbt]
+fun_induction isMinHeap; all_goals (grind [rootIsMinOfChildren])
 
-lemma leftAndRightAreMinHeapLeft (l: BinaryTree ℕ) (r: BinaryTree ℕ) (v: ℕ): leftAndRightAreMinHeap (node l v r) → leftAndRightAreMinHeap l := by
+
+lemma leftAndRightAreMinHeapAndRootIsMinOfChildrenToMinHeap (bt: BinaryTree ENat): leftAndRightAreMinHeap bt ∧ rootIsMinOfChildren bt → isMinHeap bt := by
+intro hbt
+fun_induction isMinHeap; all_goals (simp [rootIsMinOfChildren, leftAndRightAreMinHeap] at hbt;simp[hbt])
+
+lemma leftAndRightAreMinHeapLeft (l: BinaryTree ENat) (r: BinaryTree ENat) (v: ENat): leftAndRightAreMinHeap (node l v r) → leftAndRightAreMinHeap l := by
 intro hbt
 simp [leftAndRightAreMinHeap] at hbt
 simp [minHeapThenLeftAndRightAreMinHeap, hbt]
 
 
-lemma leftAndRightAreMinHeapRight (l: BinaryTree ℕ) (r: BinaryTree ℕ) (v: ℕ): leftAndRightAreMinHeap (node l v r) = true → leftAndRightAreMinHeap r =true := by
+lemma leftAndRightAreMinHeapRight (l: BinaryTree ENat) (r: BinaryTree ENat) (v: ENat): leftAndRightAreMinHeap (node l v r)  → leftAndRightAreMinHeap r := by
 intro hbt
 simp [leftAndRightAreMinHeap] at hbt
 simp [minHeapThenLeftAndRightAreMinHeap, hbt]
 
-lemma heapifyPreservesStructure (bt: BinaryTree ℕ): (∃ l r v, bt = node l v r) →  ∃ l' v' r', heapify bt = node l' v' r' := by
+lemma heapifyPreservesStructure (bt: BinaryTree ENat): (∃ l r v, bt = node l v r) →  ∃ l' v' r', heapify bt = node l' v' r' := by
 intro hbt
 fun_induction heapify; all_goals expose_names
 . obtain ⟨l, r, v, hbt⟩ := hbt
   contradiction
 all_goals simp
 
+def min:  BinaryTree ENat → ENat
+| leaf => ⊤
+| node l v r => match l, r with
+    | leaf, leaf => v
+    | leaf, node _ rv _ => if v <= rv then v else rv
+    | node _ lv _, leaf => if v <= lv then v else lv
+    | node _ lv _, node _ rv _ =>  if lv <= rv then
+                                     if v <= lv then v
+                                     else lv
+                                    else
+                                      if v <= rv then v
+                                      else rv
 
 
-def contains: (BinaryTree ℕ) → ℕ → Prop
+lemma heapifyPreservesStructureAndRootMin (bt: BinaryTree ENat): (∃ l r v, bt = node l v r) →  ∃ l' v' r', heapify bt = node l' v' r' ∧ v' ≤ (min bt) := by
+intro hbt
+fun_induction heapify; all_goals expose_names
+. obtain ⟨l, r, v, hbt⟩ := hbt
+  contradiction
+all_goals grind [min]
+
+def contains: (BinaryTree ENat) → ENat → Prop
 | leaf, _ => false
 | node l v r, v' => v=v' ∨ contains l v' ∨ contains r v'
 
@@ -97,76 +102,203 @@ def contains: (BinaryTree ℕ) → ℕ → Prop
 --all_goals sorry
 
 
-lemma heapifyPreservesMembers (bt: BinaryTree ℕ) (v: ℕ): contains bt v → contains (heapify bt) v := by
+lemma heapifyPreservesMembers (bt: BinaryTree ENat) (v: ENat): contains bt v → contains (heapify bt) v := by
 intro hbt
 fun_induction heapify generalizing v; all_goals try grind[contains]
 
-lemma containsIsNode (bt: BinaryTree ℕ) (v: ℕ): contains bt v → ∃ l v' r, bt = node l v' r := by
+lemma containsIsNode (bt: BinaryTree ENat) (v: ENat): contains bt v → ∃ l v' r, bt = node l v' r := by
 fun_induction contains; all_goals simp
 
-lemma minHeapMemberLeRoot (bt: BinaryTree ℕ) (v v': ℕ):  isMinHeap bt → (∃ l v'' r, bt = (node l v'' r) ∧ v'' ≤ v) →  contains bt v' → v' ≤ v := by
-intro hmin hl hc
-fun_induction contains generalizing v
+lemma minHeapRootMin (bt l r: BinaryTree ENat) (v: ENat): bt = (node l v r) → isMinHeap bt → v = min bt := by
+intro hbt hmin
+fun_induction isMinHeap; all_goals grind [min]
+
+
+lemma minHeapMemberLeRoot (bt: BinaryTree ENat) (v: ENat):  isMinHeap bt →  contains bt v → v ≤ min bt := by
+intro hmin hl
+fun_induction contains
 . contradiction
 . expose_names
-  cases hc; all_goals expose_names
-  . obtain ⟨v'', l', r', h⟩ := h
-    have: v_1 ≤ v := by grind
-    grind
-  . cases h; all_goals expose_names
-    . apply ih2
-      . apply minHeapThenLeftAndRightAreMinHeap at hmin
-        simp [leftAndRightAreMinHeap] at hmin
-        simp [hmin]
-      .
-
-
-    . cases l
-      . contradiction
-      . expose_names
-        have: l = a.node a_1 a_2
-
-
-lemma heapifyEstablishesRootIsMinOfChildren (bt: BinaryTree ℕ) (hbt: leftAndRightAreMinHeap bt): rootIsMinOfChildren (heapify bt) := by
-fun_induction heapify; all_goals expose_names; all_goals try grind[rootIsMinOfChildren, leftAndRightAreMinHeap]
-. have hr: (rl.node rv rr).leftAndRightAreMinHeap := by
-    grind [leftAndRightAreMinHeapRight]
-  simp [leftAndRightAreMinHeap] at hr
-  simp [leftAndRightAreMinHeap] at ih1
-  obtain ⟨hr1, hr2⟩ := hr
-  apply ih1 at hr1
-  apply hr1 at hr2
-  have: ∃ l' v' r', heapify (node rl v rr) = node l' v' r' := by
-    simp [heapifyPreservesStructure (node rl v rr)]
-  obtain ⟨rl', v', rr', hrw⟩ := this
-  rw [hrw]
-  simp[rootIsMinOfChildren]
-  grw[h]
-  rw [hrw] at hr2
-  have: contains (node rl' v' rr') v := by
-    rw [←hrw]
-    apply heapifyPreservesMembers
-    simp [contains]
-
-
-
+  cases hl
+  . sorry
   sorry
-all_goals sorry
+  -- cases hc; all_goals expose_names
+  -- . obtain ⟨v'', l', r', h⟩ := h
+  --   have: v_1 ≤ v := by grind
+  --   grind
+  -- . cases h; all_goals expose_names
+  --   . apply ih2
+  --     . apply minHeapThenLeftAndRightAreMinHeap at hmin
+  --       simp [leftAndRightAreMinHeap] at hmin
+  --       simp [hmin]
+  --     . sorry
 
-lemma heapifyEstablishesLeftAndRigthAreMinHeap (bt: BinaryTree ℕ) (hbt: leftAndRightAreMinHeap bt): leftAndRightAreMinHeap (heapify bt) := by
-fun_induction heapify; all_goals expose_names
-. simp [leftAndRightAreMinHeap]
-. simp [leftAndRightAreMinHeap, isMinHeap]
-. simp [leftAndRightAreMinHeap, isMinHeap]
+
+--     . cases l
+--       . contradiction
+--       . expose_names
+--         have: l = a.node a_1 a_2
+
+
+-- lemma heapifyEstablishesRootIsMinOfChildren (bt: BinaryTree ENat) (hbt: leftAndRightAreMinHeap bt): rootIsMinOfChildren (heapify bt) := by
+-- fun_induction heapify; all_goals expose_names; all_goals try grind[rootIsMinOfChildren, leftAndRightAreMinHeap]
+-- .
+--  have hr: (rl.node rv rr).leftAndRightAreMinHeap := by
+--     grind [leftAndRightAreMinHeapRight]
+--   simp [leftAndRightAreMinHeap] at hr
+--   simp [leftAndRightAreMinHeap] at ih1
+--   obtain ⟨hr1, hr2⟩ := hr
+--   apply ih1 at hr1
+--   apply hr1 at hr2
+--   have: ∃ l' v' r', heapify (node rl v rr) = node l' v' r' := by
+--     simp [heapifyPreservesStructure (node rl v rr)]
+--   obtain ⟨rl', v', rr', hrw⟩ := this
+--   rw [hrw]
+--   simp[rootIsMinOfChildren]
+--   grw[h]
+--   rw [hrw] at hr2
+--   have: contains (node rl' v' rr') v := by
+--     rw [←hrw]
+--     apply heapifyPreservesMembers
+--     simp [contains]
+
+
+
+--   sorry
+-- all_goals sorry
+
+-- lemma heapifyEstablishesLeftAndRigthAreMinHeap (bt: BinaryTree ENat) (hbt: leftAndRightAreMinHeap bt): leftAndRightAreMinHeap (heapify bt) := by
+-- fun_induction heapify; all_goals expose_names
+-- . simp [leftAndRightAreMinHeap]
+-- . simp [leftAndRightAreMinHeap, isMinHeap]
+-- . simp [leftAndRightAreMinHeap, isMinHeap]
+--   simp [leftAndRightAreMinHeap] at hbt
+--   have hbtr: (rl.node rv rr).leftAndRightAreMinHeap := by grind [←minHeapThenLeftAndRightAreMinHeap]
+--   apply ih1 at hbtr
+--   sorry
+-- all_goals sorry
+
+--lemma leftAndRightAreMinHeapAndRootIsMinImpliesIsHeap ()
+
+lemma heapifyPreservesMinHeap (bt: BinaryTree ENat): isMinHeap bt → bt = heapify bt := by
+fun_induction heapify; all_goals expose_names; all_goals try grind
+. intro hbt
+  by_contra
+  have hbtmin: v = min (leaf.node v (rl.node rv rr)) := by grind [minHeapRootMin]
+  grind[min]
+. intro hbt
+  by_contra
+  have hbtmin: v = min ((ll.node lv lr).node v leaf) := by grind [minHeapRootMin]
+  grind[min]
+. intro hbt
+  have hbtmin: v = min ((ll.node lv lr).node v (rl.node rv rr)) := by grind [minHeapRootMin]
+  grind[min]
+. intro hbt
+  have hbtmin: v = min ((ll.node lv lr).node v (rl.node rv rr)) := by grind [minHeapRootMin]
+  grind[min]
+
+lemma binTreeEq (l r l' r': BinaryTree ENat) (v v': ENat): (node l v r) = (node l' v' r') → r = r' := by
+grind only
+
+lemma decreaseRootIsHeap (l r: BinaryTree ENat) (v v': ENat): isMinHeap (node l v r) →  v' ≤ min (node l v r) → isMinHeap (node l v' r) := by sorry
+
+lemma heapifyEstablishesMinHeap' (bt l r: BinaryTree ENat) (v: ENat): bt = node l v r ∧  isMinHeap l ∧ isMinHeap r → isMinHeap (heapify bt) := by
+fun_induction heapify generalizing l r v; all_goals expose_names
+. simp [isMinHeap]
+. simp [isMinHeap]
+. intro ⟨hr, hminl, hminr⟩
+  apply leftAndRightAreMinHeapAndRootIsMinOfChildrenToMinHeap
+  have: ∃ rl' v' rr', (rl.node v_1 rr).heapify = node rl' v' rr' ∧ v' ≤ min (rl.node v_1 rr) := by
+        apply heapifyPreservesStructureAndRootMin
+        simp
+  obtain ⟨rl', v', rr', hr1, hr2⟩ := this
+  have hv: v=v_1 := by grind
+  have hrnode: r = (rl.node rv rr) := by
+        apply binTreeEq at hr
+        simp [hr]
+  constructor
+  . simp [leftAndRightAreMinHeap]
+    constructor
+    . simp [isMinHeap]
+    . specialize ih1 rl rr v_1
+      simp at ih1
+      apply minHeapThenLeftAndRightAreMinHeap at hminr
+      simp [leftAndRightAreMinHeap] at hminr
+      simp [hrnode] at hminr
+      apply ih1; all_goals grind
+  . rw [hr1]
+    simp [rootIsMinOfChildren]
+    have hrvmin : rv = min (rl.node rv rr) := by sorry
+    have hcontains: contains (rl.node rv rr) v' ∨ v'= v_1 := by sorry
+    cases hcontains
+    . expose_names
+      apply minHeapMemberLeRoot r v' at hminr
+      rw [← hrnode] at h_1
+      apply hminr at h_1
+      sorry
+    . expose_names
+      rw [h_1]
+      grw [h]
+
+
+
+. grind [isMinHeap]
+. sorry
+. grind [isMinHeap]
+. grind [isMinHeap]
+. sorry
+. grind [isMinHeap]
+. sorry
+
+
+  -- have: ∃ rl' v' rr', (rl.node v_1 rr).heapify = node rl' v' rr' ∧ v' ≤ min (rl.node v_1 rr) := by
+  --     apply heapifyPreservesStructureAndRootMin
+  --     simp
+  -- obtain ⟨rl', v', rr', hr1, hr2⟩ := this
+  -- rw [hr1]
+  -- apply leftAndRightAreMinHeapAndRootIsMinOfChildrenToMinHeap
+  -- constructor
+  -- . simp [leftAndRightAreMinHeap]
+  --   constructor
+  --   . simp [isMinHeap]
+  --   . rw [← hr1]
+  --     apply ih1
+  --     simp [hr]
+  --     have: r = (rl.node rv rr) := by
+  --       apply binTreeEq at hr
+  --       simp [hr]
+
+  --     apply decreaseRootIsHeap rl' rr' v_1
+
+
+--   .
+
+
+
+
+
+
+lemma heapifyEstablishesMinHeap (bt: BinaryTree ENat): (hbt: leftAndRightAreMinHeap bt) → isMinHeap (heapify bt) := by
+fun_induction heapify; all_goals expose_names; all_goals try grind [isMinHeap]
+. intro hbt
   simp [leftAndRightAreMinHeap] at hbt
-  have hbtr: (rl.node rv rr).leftAndRightAreMinHeap := by grind [←minHeapThenLeftAndRightAreMinHeap]
-  apply ih1 at hbtr
-  sorry
-all_goals sorry
+  obtain ⟨hb1, hb2⟩ := hbt
+  apply minHeapThenLeftAndRightAreMinHeap at hb2
+  apply ih1 at hb2
+  apply leftAndRightAreMinHeapAndRootIsMinOfChildrenToMinHeap
+  constructor
+  . simp [leftAndRightAreMinHeap]
+    constructor
+    . simp [isMinHeap]
+    . exact hb2
+  .
+    have: ∃ rl' v' rr', (rl.node v rr).heapify = node rl' v' rr' ∧ v' ≤ min (rl.node v rr) := by
+      apply heapifyPreservesStructureAndRootMin
+      simp
+    obtain ⟨rl', v', rr', hr1, hr2⟩ := this
+    rw [hr1]
 
+    have: rv <= v' := by sorry
 
-lemma heapifyEstablishesMinHeap (bt: BinaryTree ℕ) (hbt: leftAndRigthAreMinHeap bt): isMinHeap (heapify bt) := by
-fun_induction heapify; all_goals expose_names
-. simp [isMinHeap]
-. simp [isMinHeap]
-all_goals sorry
+    simp[rootIsMinOfChildren]
+    exact this
